SrcTranslated/TypesExternal.lean
@@ -18,7 +18,7 @@ set_option maxHeartbeats 1000000
     Source: '/rustc/library/core/src/num/error.rs', lines 10:0-10:26
     Name pattern: [core::num::error::TryFromIntError] -/
 @[rust_type "core::num::error::TryFromIntError"]
-axiom core.num.error.TryFromIntError : Type
+structure core.num.error.TryFromIntError deriving Inhabited, DecidableEq
 
 /-- [alloc::collections::vec_deque::into_iter::IntoIter]
     Source: '/rustc/library/alloc/src/collections/vec_deque/into_iter.rs', lines 18:0-21:1
